StrictPositivityLemma.v
@@ -84,7 +84,7 @@ Ltac apply_induction H :=
   match goal with
     H2: forall_implies (fun _ => reducible_values _ _ ?A) ?ptheta ?theta' |-
       reducible_values (?theta' ++ _) _ ?T =>
-      apply H with (typeNodes T, index T) ptheta A
+      apply H with (get_measure T) ptheta A
   end.
 
 Ltac find_exists3 :=
@@ -113,7 +113,7 @@ Definition sp_push_forall_prop T: Prop :=
     forall_implies (fun a => reducible_values theta a A) pre_theta theta' ->
     reducible_values (theta' ++ theta) v T.
 
-Definition sp_push_forall_prop_aux m T: Prop := (typeNodes T, index T) = m -> sp_push_forall_prop T.
+Definition sp_push_forall_prop_aux m T: Prop := get_measure T = m -> sp_push_forall_prop T.
 
 Definition sp_push_forall_until m: Prop := forall m', m' << m -> forall T', sp_push_forall_prop_aux m' T'.
 
@@ -154,7 +154,7 @@ Ltac t_spos_proof HH :=
       ( progress unfold reduces_to in * ) ||
       find_smallstep_value ||
       apply strictly_positive_open ||
-      apply left_lex ||
+      apply leq_lt_measure ||
       find_exists ||
       find_exists3 ||
       find_exists2 || (* must be after find_exists3 *)
@@ -313,7 +313,7 @@ Proof.
   apply_induction H;
     repeat
       step || t_valid_interpretation_equiv || t_forall_implies_equiv ||
-      apply left_lex ||
+      apply leq_lt_measure ||
       (progress autorewrite with bsize in * ) ||
       apply strictly_positive_swap ||
       apply twf_topen ||
@@ -412,10 +412,10 @@ Proof.
       | H1: non_empty ?theta ?A,
         H2: forall_implies _ ?ptheta ?theta' |-
           reducible_values (((?X, fun t => reducible_values (?theta' ++ ?theta) t ?R) :: ?theta') ++ ?theta) _ ?T =>
-          apply H with (typeNodes T, index T) ((X, fun a t => reducible_values (push_one a pre_theta ++ theta) t R) :: ptheta) A
+          apply H with (get_measure T) ((X, fun a t => reducible_values (push_one a pre_theta ++ theta) t R) :: ptheta) A
       end;
         repeat
-          step || apply left_lex || autorewrite with bsize in * || t_deterministic_star ||
+          step || apply leq_lt_measure || autorewrite with bsize in * || t_deterministic_star ||
           apply is_erased_type_topen || t_instantiate_reducible ||
           apply wf_topen || apply twf_topen || apply reducibility_is_candidate ||
           (poseNew (Mark 0 "strictly_positive_topen2"); apply strictly_positive_topen2);
@@ -433,13 +433,21 @@ Proof.
             try finisher.
       + (* We apply one last time the induction hypothesis for rec(n) *)
         apply_induction H;
-          repeat step || apply right_lex || simp_spos; eauto using lt_index_step;
+          repeat step || apply right_lex, right_lex || simp_spos; eauto using lt_index_step;
             eauto with bwf btwf berased.
 Qed.
 
 Hint Immediate sp_push_forall_rec: b_push.
 
-Lemma strictly_positive_push_forall_aux: forall m T, sp_push_forall_prop_aux m T.
+Lemma sp_push_forall_interpret:
+  forall m T, sp_push_forall_until m -> sp_push_forall_prop_aux m (T_interpret T).
+Proof.
+  repeat autounfold with u_push; steps.
+Qed.
+
+Hint Immediate sp_push_forall_interpret: b_push.
+
+Lemma strictly_positive_push_forall_aux: forall (m: measure_domain) T, sp_push_forall_prop_aux m T.
 Proof.
   induction m using measure_induction; destruct T;
     eauto 2 with b_push;
